Splinter/BlockLayer/Bundle.i.dfy
@@ -1,1 +1,2 @@
 include "BlockCoordinationSystemRefinement.i.dfy"
+include "../Betree/PagedBetreeRefinement.i.dfy"
